LambdaGraph/Lemmas.lean
@@ -1,0 +1,37 @@
+import LambdaGraph.Basic
+
+theorem value_types_cn {L : Type} {p : Program L} {Γ : List L} {v : Expr L}
+  {t : Ty} (ht : p / Γ ⊢ v : t.cn) (hv : v.Value) : ∃ l σ, v = .clos l σ := by
+  rcases hv with ⟨l, σ⟩ | b
+  · exists l, σ
+  · cases ht
+
+theorem value_types_bool {L : Type} {p : Program L} {Γ : List L} {v : Expr L}
+  (ht : p / Γ ⊢ v : .bool) (hv : v.Value) : ∃ b, v = .bool b := by
+  rcases hv with ⟨l, σ⟩ | b
+  · cases ht
+  · exists b
+
+theorem progress {L : Type} [DecidableEq L] {p : Program L} {e : Expr L}
+  {t : Ty} (h : p / [] ⊢ e : t) : e.Value ∨ ∃ e', p / e ⇒ e' := by
+  generalize hΓ : [] = Γ at h
+  induction h with subst hΓ
+  | var Γ l hl => simp at hl
+  | fnRec Γ l hl => simp at hl
+  | fnNew Γ l hl h ih => right; repeat constructor
+  | app Γ f e t hf he ihf ihe =>
+    right
+    rcases ihf rfl with hvf | ⟨f', hsf⟩
+    · rcases ihe rfl with hve | ⟨e', hse⟩
+      · obtain ⟨l, σ, rfl⟩ := value_types_cn hf hvf
+        exact ⟨_, Step.app _ _ _ hve⟩
+      · exact ⟨_, Step.appR _ _ _ hvf hse⟩
+    · exact ⟨_, Step.appL _ _ _ hsf⟩
+  | clos Γ l σ h ih => left; constructor
+  | bool Γ b => left; constructor
+  | cond Γ c et ef t hc het hef ihc ihet ihef =>
+    right
+    rcases ihc rfl with hvc | ⟨c', hsc⟩
+    · obtain ⟨b, rfl⟩ := value_types_bool hc hvc
+      cases b <;> repeat constructor
+    · exact ⟨_, Step.condC _ _ _ _ hsc⟩
